% vim: nu expandtab shiftwidth=2 softtabstop=2 autoindent foldmethod=marker
%%%%%%%%%%%%%%%%%%%%%%%%%%%%%%%%%%%%%%%%%%%%%%%%%%%%%%%%%%%%%%%%%%%%%%%%%%%%%
% Answers - ACB
%%%%%%%%%%%%%%%%%%%%%%%%%%%%%%%%%%%%%%%%%%%%%%%%%%%%%%%%%%%%%%%%%%%%%%%%%%%%%
\section{Answers - Factoring - ACB}
Factor and solve each equation. \\
\begin{enumerate}
%%%% 1  %%%%
\item $2x^{2} + 20x + 42 = 0$
  \begin{itemize}
  \item $A=2, B=20, C=42$
  \item $2x^{2}+14x+6x+42$
  \item $2x(x+7)+6(x+7)$
  \item $(2x+6)(x+7)$
  \end{itemize}
%%%% 2  %%%%
\item $2x^{2} + x - 3 = 0$
  \begin{itemize}
  \item $A=2, B=1, C=-3$
  \item $2x^{2}+3x-2x-3$
  \item $x(2x+3)-1(2x+3)$
  \item $(x-1)(2x+3)$
  \end{itemize}
%%%% 3  %%%%
\item $3x^{2} + 2x - 8 = 0$
  \begin{itemize}
  \item $A=3, B=2, C=-8$
  \item $3x^{2}+6x-4x-8$
  \item $3x(x+2)-4(x+2)$
  \item $(3x-4)(x+2)$
  \end{itemize}
%%%% 4  %%%%
\item $4x^{2} - 12x - 7 = 0$
  \begin{itemize}
  \item $A=4, B=-12, C=-7$
  \item $4x^{2}-14x+2x-7$
  \item $2x(x-7)+1(2x-7)$
  \item $(2x+1)(2x-7)$
  \end{itemize}
%%%% 5  %%%%
\item $2x^{2} + 5x - 12 = 0$
  \begin{itemize}
  \item $A=2, B=5, C=-12$
  \item $2x^{2}+8x-3x-12$
  \item $2x(x+4)-3(x+4)$
  \item $(2x-3)(x+4)$
  \end{itemize}
%%%% 6  %%%%
\item $2x^{2} + 9x + 9 = 0$
  \begin{itemize}
  \item $A=2, B=9, C=9$
  \item $2x^{2}+6x+3x+9$
  \item $2x(x+3)+3(x+3)$
  \item $(2x+3)(x+3)$
  \end{itemize}
%%%% 7  %%%%
\item $6x^{2} - 5x - 6 = 0$
  \begin{itemize}
  \item $A=6, B=-5, C=-6$
  \item $6x^{2}-9x+4x-6$
  \item $3x(2x-3)+2(2x-3)$
  \item $(3x+2)(2x-3)$
  \end{itemize}
%%%% 8  %%%%
\item $4x^{2} - 7x + 3 = 0$
  \begin{itemize}
  \item $A=4, B=-7, C=3$
  \item $4x^{2}-3x-4x+3$
  \item $x(4x-3)-1(4x-3)$
  \item $(x-1)(4x-3)$
  \end{itemize}
%%%% 9  %%%%
\item $4x^{2} + 4x - 3 = 0$
  \begin{itemize}
  \item $A=4, B=4, C=-3$
  \item $4x^{2}+6x-2x-3$
  \item $2x(2x+3)-1(2x+3)$
  \item $(2x-1)(2x+3)$
  \end{itemize}
%%%% 10 %%%%
\item $3x^{2} + 13x + 12 = 0$
  \begin{itemize}
  \item $A=3, B=13, C=12$
  \item $3x^{2}+9x+4x+12$
  \item $3x(x+3)+4(x+3)$
  \item $(3x+4)(x+3)$
  \end{itemize}
%%%% 11 %%%%
\item $4x^{2} - 15x - 4 = 0$
  \begin{itemize}
  \item $A=4, B=-15, C=-4$
  \item $4x^{2}-16x+x-4$
  \item $4x(x-4)+1(x-4)$
  \item $(4x+1)(x-4)$
  \end{itemize}
%%%% 12 %%%%
\item $4x^{2} - 16x + 15 = 0$
  \begin{itemize}
  \item $A=4, B=-16, C=15$
  \item $4x^{2}-10x-6x+15$
  \item $2x(2x-5)-3(2x-5)$
  \item $(2x-3)(2x-5)$
  \end{itemize}
%%%% 13 %%%%
\item $6x^{2} + 10x - 24 = 0$
  \begin{itemize}
  \item $2(3x^{2}+5x-12$
  \item $A=3, B=5, C=-12$
  \item $2(3x^{2}+9x-4x-12)$
  \item $2(3x(x+3)-4(x+3))$
  \item $2(3x-4)(x+3)$
  \end{itemize}
%%%% 14 %%%%
\item $2x^{2} - x - 6 = 0$
  \begin{itemize}
  \item $A=2, B=-1, C=-6$
  \item $2x^{2}-4x+3x-6$
  \item $2x(x-2)+3(x-2)$
  \item $(2x+3)(x-2)$
  \end{itemize}
%%%% 15 %%%%
\item $4x^{2} + 12x + 5 = 0$
  \begin{itemize}
  \item $A=4, B=12, C=5$
  \item $4x^{2}+2x+10x+5$
  \item $2x(2x+1)+5(2x+1)$
  \item $(2x+5)(2x+1)$
  \end{itemize}
%%%% 16 %%%%
\item $3x^{2} - 25x + 28 = 0$
  \begin{itemize}
  \item $A=3, B=-25, C=28$
  \item $3x^{2}-4x-21x+28$
  \item $x(3x-4)-7(3x-4)$
  \item $(x-7)(3x-4)$
  \end{itemize}
%%%% 17 %%%%
\item $3x^{2} - x - 14 = 0$
  \begin{itemize}
  \item $A=3, B=-1, C=-14$
  \item $3x^{2}-7x+6x-14$
  \item $x(3x-7)+2(3x-7)$
  \item $(x+2)(3x-7)$
  \end{itemize}
%%%% 18 %%%%
\item $6x^{2} + 4x - 42 = 0$
  \begin{itemize}
  \item $2(3x^{2}+2x-21)$
  \item $A=3, B=2, C=-21$
  \item $2(3x^{2}+9x-7x-21)$
  \item $2(3x(x+3)-7(x+3))$
  \item $2(3x-7)(x+3)$
  \end{itemize}
%%%% 19 %%%%
\item $3x^{2} + 7x - 6 = 0$
  \begin{itemize}
  \item $A=3, B=7, C=-6$
  \item $3x^{2}+9x-2x-6$
  \item $3x(x+3)-2(x+3)$
  \item $(3x-2)(x+3)$
  \end{itemize}
%%%% 20 %%%%
\item $4x^{2} - 4x - 3 = 0$
  \begin{itemize}
  \item $A=4, B=-4, C=-3$
  \item $4x^{2}-6x+2x-3$
  \item $2x(2x-3)+1(2x-3)$
  \item $(2x+1)(2x-3)$
  \end{itemize}
%%%% 21 %%%%
\item $3x^{2} + 22x - 45 = 0$
  \begin{itemize}
  \item $A=3, B=22, C=-45$
  \item $3x^{2}+27x-5x-45$
  \item $3x(x+9)-5(x+9)$
  \item $(3x-5)(x+9)$
  \end{itemize}
%%%% 22 %%%%
\item $4x^{2} - 8x - 21 = 0$
  \begin{itemize}
  \item $A=4, B=-8, C=-21$
  \item $4x^{2}-14x+6x-21$
  \item $2x(x-7)+3(2x-7)$
  \item $(2x+3)(2x-7)$
  \end{itemize}
%%%% 23 %%%%
\item $2x^{2} + 9x - 35 =0$
  \begin{itemize}
  \item $A=2, B=9, C=-35$
  \item $2x^{2}+14x-5x-35$
  \item $2x(x+7)-5(x+5)$
  \item $(2x-5)(x+7)$
  \end{itemize}
%%%% 24 %%%%
\item $9x^{2} + 24x - 20 = 0$
  \begin{itemize}
  \item $A=9, B=24, C=-20$
  \item $9x^{2}+30x-6x-20$
  \item $3x(3x+10)-2(3x+10)$
  \item $(3x-2)(3x+10)$
  \end{itemize}
%%%% 25 %%%%
\item $2x^{2} + 11x - 40 = 0$
  \begin{itemize}
  \item $A=2, B=11, C=-40$
  \item $2x^{2}+16x-5x-40$
  \item $2x(x+8)-5(x+8)$
  \item $(2x-5)(x+8)$
  \end{itemize}
\end{enumerate}
